\question % Sample Questions 2, Q7.
Let $k$, $a$, $b$ and $c$ be real numbers. Consider the polynomial
\[
    P(x) = (x + 2)(kx^3 + ax^2 + bx + c) + (-7x + 22).
\]
It's known that $x + 1$ is a factor and $x = 2$ is a zero of $P(x)$. Moreover, when $P(x)$ is divided by $x - 3$, the remainder is $56$.

\begin{parts}

\part[3]
Show that an augmented matrix for the coefficients $a$, $b$ and $c$ can be written as
\[
	\begin{amatrix}{3}
        1 & -1 & 1 & k - 29 \\
        4 & 2 & 1 & -8k - 2 \\
        9 & 3 & 1 & -27k + 11
    \end{amatrix}
\]

\begin{EnvFullwidth}
\begin{solutionorgrid}[1.5in]
We have $P(-1) = 0$, so
\begin{align}
    (-1 + 2)(k \times (-1) + a \times 1 + b \times (-1) + c) + (-7 \times (-1) + 22) &= 0 \notag \\
    a - b + c &= k - 29.
\end{align}
Similarly, $P(2) = 0$, so
\begin{align}
    (2 + 2)(k \times 8 + a \times 4 + b \times 2 + c) + (-7 \times 2 + 22) &= 0 \notag \\
    16a + 8b + 4c &= -32k - 8 \notag \\
    4a + 2b + c &= -8k - 2.
\end{align}
But since $P(3) = 56$ we get
\begin{align}
    (3 + 2)(k \times 27 + a \times 9 + b \times 3 + c) + (-7 \times 3 + 22) &= 56 \notag \\
    \cancel{5 \times} (k \times 27 + a \times 9 + b \times 3 + c) &= \cancel{5 \times} 11 \notag \\
    9a + 3b + c &= -27k + 11.
\end{align}
\end{solutionorgrid}
\end{EnvFullwidth}

\part[4]
Clearly showing all row operations, show that
\[
    a = -4k + 1, \qquad b = k + 8, \qquad c = 6k - 22.
\]

\begin{EnvFullwidth}
\begin{solutionorgrid}[4.5in]
By Gaussian elimination
\begin{align*}
	\begin{amatrix}{3}
        1 & -1 & 1 & k - 29 \\
        4 & 2 & 1 & -8k - 2 \\
        9 & 3 & 1 & -27k + 11
    \end{amatrix}
    &\sim
	\begin{amatrix}{3}
        1 & -1 & 1 & k - 29 \\
        0 & -6 & 3 & 12k - 114 \\
        0 & -12 & 8 & 36k - 272
    \end{amatrix}
    &&
    \begin{array}{l}
 	    \\
	    R_2 \to 4R_1 - R_2 \\
	    R_3 \to 9R_1 - R_3 
    \end{array} \\
%     &\sim
% 	\begin{amatrix}{3}
%         1 & -1 & 1 & k - 29 \\
%         0 & 1 & -\frac{1}{2} & -2k + 19 \\
%         0 & 3 & -2 & -9k + 68
%     \end{amatrix}
%     &&
%     \begin{array}{l}
%  	    \\
% 	    R_2 \to -\frac{1}{6}R_2 \\
% 	    R_3 \to -\frac{1}{4}R_3
%     \end{array} \\
    &\sim
	\begin{amatrix}{3}
        1 & -1 & 1 & k - 29 \\
        0 & 1 & -\frac{1}{2} & -2k + 19 \\
        0 & 0 & 1 & 6k - 22
    \end{amatrix}
    &&
    \begin{array}{l}
 	    \\
 	    R_2 \to -\frac{1}{6} R_2 \\
	    R_3 \to 6R_2 - 2R_3
    \end{array} \\
    &\sim
	\begin{amatrix}{3}
        1 & 0 & \frac{1}{2} & -k - 10 \\
        0 & 2 & 0 & 2k + 16 \\
        0 & 0 & 1 & 6k - 22
    \end{amatrix}
    &&
    \begin{array}{l}
 	    R_1 \to R_1 + R_2 \\
	    R_2 \to 2R_2 + R_3 \\
	    \\
    \end{array} \\
    &\sim
	\begin{amatrix}{3}
        2 & 0 & 0 & -8k + 2 \\
        0 & 1 & 0 & k + 8 \\
        0 & 0 & 1 & 6k - 22
    \end{amatrix}
    &&
    \begin{array}{l}
 	    R_1 \to 2R_1 - R_3 \\
	    R_2 \to \frac{1}{2}R_2 \\
	    \\
    \end{array} \\
    &\sim
	\begin{amatrix}{3}
        1 & 0 & 0 & -4k + 1 \\
        0 & 1 & 0 & k + 8 \\
        0 & 0 & 1 & 6k - 22
    \end{amatrix}
    &&
    \begin{array}{l}
 	    R_1 \to \frac{1}{2}R_1 \\
	    \\
	    \\
    \end{array}
\end{align*}
\end{solutionorgrid}
\end{EnvFullwidth}

\part[1]
Hence, find $P(x)$ for $k = 2$. (There's no need to simplify $P(x)$.)

\begin{EnvFullwidth}
\begin{solutionorgrid}[1in]
If $k = 2$, then
\[
    a = -7, \qquad b = 10, \qquad c = -10.
\]
Thus,
\[
    P(x) = (x + 2)(2x^3 - 7x^2 + 10x - 10) + (-7x + 22).
\]
(For what it's worth, $P(x) = 2x^4 - 3x^3 - 4x^2 + 3x + 2$.)
\end{solutionorgrid}
\end{EnvFullwidth}

\end{parts}
